\customchapter[January 9, 2023]{Lecture 2: Grammer}
	\begin{theorem}{}
		$\left| uv \right| = \left| u \right| + \left| v \right|$.
	\end{theorem}

	\begin{proof}
		We will use mathematical induction to prove this. \\
		\textbf{Base case:} $\left| \lm v \right| = \left| v \right| = \left| \lm \right| + \left| v \right|$. \\
		\textbf{Inductive step:} Assume $\left| uv \right| = \left| u \right| + \left| v \right|$. Then $\left| u'v \right| = \left| u' \right| + \left| v \right| = \left| u \right| + \left| v \right| + 1$. \\
		Thus, $\left| uv \right| = \left| u'v \right| = \left| u \right| + \left| v \right| + 1 = \left| u \right| + \left| v \right|$. \\
		Thus, $\left| uv \right| = \left| u \right| + \left| v \right|$.
		\\ $\square$
	\end{proof}

	\section{Grammer}
	\begin{definition}{Grammer}
		A grammer $\bbG = \{\bbV, \bbT, \bbS, \bbP\}$ 
		\begin{itemize}
			\item $\bbV$ is finite set of objects called variables. 
			\item $\bbT$ is finite st of objects called terminals. 
			\item $\bbS \in \bbV$: special symbol called start variable 
			\item $\bbP$ is a finite set of rules 
		\end{itemize}
	\end{definition}	
